generational/spec/GC.Gen.HeapInvariant.fsti
@@ -152,6 +152,16 @@ val minor_major_fields_no_blue_intro (minor: minor_state) (major: heap)
               ~(is_blue ((minor_read_field minor obj j) <: obj_addr) major)))
           (ensures minor_major_fields_no_blue minor major)
 
+val minor_major_fields_no_blue_no_pointer_fields
+  : minor:minor_state -> major:heap ->
+    Lemma
+      (requires
+        (forall (obj:U64.t) (j:nat).
+          Seq.mem obj (minor_objects minor) /\
+          j < minor_wosize minor obj ==>
+          ~(is_pointer_field (minor_read_field minor obj j))))
+      (ensures minor_major_fields_no_blue minor major)
+
 val minor_major_fields_no_blue_elim (minor: minor_state) (major: heap)
   (obj: U64.t) (j: nat)
   : Lemma (requires minor_major_fields_no_blue minor major /\
