spot/GC.SPOT.ConcreteForwarding.fst
@@ -1,0 +1,220 @@
+module GC.SPOT.ConcreteForwarding
+
+module U64 = FStar.UInt64
+module Seq = FStar.Seq
+
+open FStar.Seq
+open GC.Spec.Base
+open GC.Gen.Base
+open GC.Gen.MinorHeap
+
+module Layout = GC.SPOT.Layout
+module ThreeObjects = GC.SPOT.ThreeObjects
+module ConcreteMinor = GC.SPOT.ConcreteMinor
+module ConcreteMajor = GC.SPOT.ConcreteMajor
+module Promote = GC.Gen.Promote
+module Cheney = GC.Gen.Cheney
+
+#push-options "--z3rlimit 10 --fuel 0 --ifuel 0"
+
+let zero_not_in_minor_objects ()
+  : Lemma (ensures ~(Seq.mem 0UL (minor_objects ConcreteMinor.spot_minor2)))
+  =
+  if Seq.mem 0UL (minor_objects ConcreteMinor.spot_minor2) then begin
+    minor_objects_valid ConcreteMinor.spot_minor2 0UL;
+    assert False
+  end
+
+let zero_not_infix ()
+  : Lemma (ensures ~(is_infix_in_minor ConcreteMinor.spot_minor2 0UL))
+  = assert_norm (is_infix_in_minor ConcreteMinor.spot_minor2 0UL == false)
+
+let c_not_minor_or_infix (r: unit{ConcreteMajor.spot_major_room})
+  : Lemma (ensures
+      ~(Seq.mem (ConcreteMajor.spot_c r <: U64.t)
+          (minor_objects ConcreteMinor.spot_minor2)) /\
+      ~(is_infix_in_minor ConcreteMinor.spot_minor2
+          (ConcreteMajor.spot_c r <: U64.t)))
+  =
+  let c = ConcreteMajor.spot_c r in
+  ConcreteMajor.spot_major_layout_facts r;
+  zero_addr_above_minor ();
+  assert (U64.v c >= minor_heap_size);
+  if Seq.mem (c <: U64.t) (minor_objects ConcreteMinor.spot_minor2) then begin
+    minor_objects_valid ConcreteMinor.spot_minor2 (c <: U64.t);
+    assert False
+  end;
+  assert (~(is_infix_in_minor ConcreteMinor.spot_minor2 (c <: U64.t)))
+
+let b_not_infix ()
+  : Lemma (ensures ~(is_infix_in_minor ConcreteMinor.spot_minor2 Layout.b_minor))
+  =
+  ConcreteMinor.spot_minor_two_object_layout ();
+  minor_objects_not_infix ConcreteMinor.spot_minor2 Layout.b_minor;
+  assert (minor_tag ConcreteMinor.spot_minor2 Layout.b_minor <> 249);
+  assert (~(is_infix_in_minor ConcreteMinor.spot_minor2 Layout.b_minor))
+
+let forward_major_c_noop
+  (r: unit{ConcreteMajor.spot_major_room})
+  (cs: Cheney.cheney_state)
+  : Lemma (ensures
+      Cheney.cheney_forward_one ConcreteMinor.spot_minor2 cs
+        (ConcreteMajor.spot_c r <: U64.t) == cs)
+  =
+  c_not_minor_or_infix r;
+  Cheney.cheney_forward_one_noop
+    ConcreteMinor.spot_minor2 cs (ConcreteMajor.spot_c r <: U64.t)
+
+let forward_zero_noop (cs: Cheney.cheney_state)
+  : Lemma (ensures Cheney.cheney_forward_one ConcreteMinor.spot_minor2 cs 0UL == cs)
+  =
+  zero_not_in_minor_objects ();
+  zero_not_infix ();
+  Cheney.cheney_forward_one_noop ConcreteMinor.spot_minor2 cs 0UL
+
+let forward_a_preserves_b (cs: Cheney.cheney_state)
+  : Lemma (requires cs.Cheney.cs_fwd Layout.a_minor == 0UL /\
+                    cs.Cheney.cs_fwd Layout.b_minor == 0UL)
+          (ensures
+            (Cheney.cheney_forward_one
+              ConcreteMinor.spot_minor2 cs Layout.a_minor).Cheney.cs_fwd
+              Layout.b_minor == 0UL)
+  =
+  ConcreteMinor.spot_minor_a_not_infix ();
+  Layout.a_b_distinct ();
+  Cheney.cheney_forward_one_normal ConcreteMinor.spot_minor2 cs Layout.a_minor;
+  Cheney.cheney_forward_normal_other_fwd
+    ConcreteMinor.spot_minor2 cs Layout.a_minor Layout.b_minor
+
+let forward_roots_b_zero (r: unit{ConcreteMajor.spot_major_room})
+  : Lemma (ensures
+      (let cs0 : Cheney.cheney_state =
+        { Cheney.cs_major = ConcreteMajor.spot_major_heap r;
+          Cheney.cs_fp = ConcreteMajor.spot_major_fp r;
+          Cheney.cs_fwd = Promote.empty_forwarding;
+          Cheney.cs_queue = Seq.empty } in
+       let roots = ThreeObjects.spot_roots (ConcreteMajor.spot_c r) in
+       (Cheney.cheney_forward_roots
+          ConcreteMinor.spot_minor2 cs0 roots 0).Cheney.cs_fwd
+          Layout.b_minor == 0UL))
+  =
+  let c = ConcreteMajor.spot_c r in
+  let roots = ThreeObjects.spot_roots c in
+  let cs0 : Cheney.cheney_state =
+    { Cheney.cs_major = ConcreteMajor.spot_major_heap r;
+      Cheney.cs_fp = ConcreteMajor.spot_major_fp r;
+      Cheney.cs_fwd = Promote.empty_forwarding;
+      Cheney.cs_queue = Seq.empty } in
+  ThreeObjects.spot_roots_len c;
+  ThreeObjects.spot_roots_index_c c;
+  ThreeObjects.spot_roots_index_a c;
+  Cheney.cheney_forward_roots_step
+    ConcreteMinor.spot_minor2 cs0 roots 0;
+  forward_major_c_noop r cs0;
+  assert (Cheney.cheney_forward_one
+    ConcreteMinor.spot_minor2 cs0 (Seq.index roots 0) == cs0);
+  Cheney.cheney_forward_roots_step
+    ConcreteMinor.spot_minor2 cs0 roots 1;
+  let cs_a = Cheney.cheney_forward_one
+    ConcreteMinor.spot_minor2 cs0 Layout.a_minor in
+  forward_a_preserves_b cs0;
+  Cheney.cheney_forward_roots_base
+    ConcreteMinor.spot_minor2 cs_a roots 2;
+  assert ((Cheney.cheney_forward_roots
+    ConcreteMinor.spot_minor2 cs0 roots 0).Cheney.cs_fwd Layout.b_minor == 0UL)
+
+let scan_after_roots_b_zero (r: unit{ConcreteMajor.spot_major_room})
+  : Lemma (ensures
+      (let cs0 : Cheney.cheney_state =
+        { Cheney.cs_major = ConcreteMajor.spot_major_heap r;
+          Cheney.cs_fp = ConcreteMajor.spot_major_fp r;
+          Cheney.cs_fwd = Promote.empty_forwarding;
+          Cheney.cs_queue = Seq.empty } in
+       let roots = ThreeObjects.spot_roots (ConcreteMajor.spot_c r) in
+       let cs_roots =
+         Cheney.cheney_forward_roots ConcreteMinor.spot_minor2 cs0 roots 0 in
+       (Cheney.cheney_scan ConcreteMinor.spot_minor2 cs_roots 0
+          (Cheney.cheney_fuel ConcreteMinor.spot_minor2)).Cheney.cs_fwd
+          Layout.b_minor == 0UL))
+  =
+  let c = ConcreteMajor.spot_c r in
+  let roots = ThreeObjects.spot_roots c in
+  let major = ConcreteMajor.spot_major_heap r in
+  let fp = ConcreteMajor.spot_major_fp r in
+  let cs0 : Cheney.cheney_state =
+    { Cheney.cs_major = major;
+      Cheney.cs_fp = fp;
+      Cheney.cs_fwd = Promote.empty_forwarding;
+      Cheney.cs_queue = Seq.empty } in
+  ThreeObjects.spot_roots_len c;
+  ThreeObjects.spot_roots_index_c c;
+  ThreeObjects.spot_roots_index_a c;
+  Cheney.cheney_forward_roots_step
+    ConcreteMinor.spot_minor2 cs0 roots 0;
+  forward_major_c_noop r cs0;
+  Cheney.cheney_forward_roots_step
+    ConcreteMinor.spot_minor2 cs0 roots 1;
+  let cs_a =
+    Cheney.cheney_forward_one ConcreteMinor.spot_minor2 cs0 Layout.a_minor in
+  forward_a_preserves_b cs0;
+  Cheney.cheney_forward_roots_base
+    ConcreteMinor.spot_minor2 cs_a roots 2;
+  assert (Cheney.cheney_forward_roots
+    ConcreteMinor.spot_minor2 cs0 roots 0 == cs_a);
+  ConcreteMinor.spot_minor_two_object_layout ();
+  ConcreteMinor.spot_minor_a_not_infix ();
+  Cheney.cheney_forward_one_normal ConcreteMinor.spot_minor2 cs0 Layout.a_minor;
+  let wz = minor_wosize ConcreteMinor.spot_minor2 Layout.a_minor in
+  assert (wz == 1);
+  let prom_a = Promote.promote_object
+    ConcreteMinor.spot_minor2 major Layout.a_minor fp wz in
+  if prom_a.Promote.new_addr = 0UL then begin
+    Cheney.cheney_forward_normal_noop_oom
+      ConcreteMinor.spot_minor2 cs0 Layout.a_minor;
+    assert (cs_a == cs0);
+    Cheney.cheney_scan_base
+      ConcreteMinor.spot_minor2 cs_a 0 (Cheney.cheney_fuel ConcreteMinor.spot_minor2)
+  end else begin
+    Cheney.cheney_forward_normal_success
+      ConcreteMinor.spot_minor2 cs0 Layout.a_minor;
+    assert (cs_a.Cheney.cs_queue ==
+      Seq.append (Seq.empty #U64.t) (Seq.create 1 Layout.a_minor));
+    assert (Seq.length cs_a.Cheney.cs_queue == 1);
+    assert (Seq.index cs_a.Cheney.cs_queue 0 == Layout.a_minor);
+    Cheney.cheney_fuel_eq ConcreteMinor.spot_minor2;
+    assert (Seq.mem Layout.a_minor (minor_objects ConcreteMinor.spot_minor2));
+    let _ = Seq.index_mem Layout.a_minor
+      (minor_objects ConcreteMinor.spot_minor2) in
+    assert (Seq.length (minor_objects ConcreteMinor.spot_minor2) > 0);
+    assert (Cheney.cheney_fuel ConcreteMinor.spot_minor2 > 0);
+    Cheney.cheney_scan_step
+      ConcreteMinor.spot_minor2 cs_a 0 (Cheney.cheney_fuel ConcreteMinor.spot_minor2);
+    ConcreteMinor.spot_minor2_field_zero Layout.a_minor 0;
+    to_minor_offset_in_minor_range 0UL;
+    assert (to_minor_offset
+      (minor_read_field ConcreteMinor.spot_minor2 Layout.a_minor 0) == 0UL);
+    Cheney.cheney_forward_fields_step
+      ConcreteMinor.spot_minor2 cs_a Layout.a_minor 0 1;
+    forward_zero_noop cs_a;
+    Cheney.cheney_forward_fields_base
+      ConcreteMinor.spot_minor2 cs_a Layout.a_minor 1 1;
+    assert (Cheney.cheney_forward_fields
+      ConcreteMinor.spot_minor2 cs_a Layout.a_minor 0 1 == cs_a);
+    Cheney.cheney_scan_base
+      ConcreteMinor.spot_minor2 cs_a 1
+      (Cheney.cheney_fuel ConcreteMinor.spot_minor2 - 1)
+  end
+
+let spot_concrete_b_forwarding_zero
+  (r: unit{ConcreteMajor.spot_major_room})
+  : Lemma (ensures
+      (Cheney.cheney_promote
+        ConcreteMinor.spot_minor2
+        (ConcreteMajor.spot_major_heap r)
+        (ConcreteMajor.spot_major_fp r)
+        (ThreeObjects.spot_roots (ConcreteMajor.spot_c r))).fwd_map
+        Layout.b_minor == 0UL)
+  =
+  scan_after_roots_b_zero r
+
+#pop-options
