spot/GC.SPOT.ConcreteForwarding.fsti
@@ -1,0 +1,20 @@
+module GC.SPOT.ConcreteForwarding
+
+module U64 = FStar.UInt64
+module Seq = FStar.Seq
+
+open FStar.Seq
+open GC.Spec.Base
+
+module Cheney = GC.Gen.Cheney
+module ConcreteMajor = GC.SPOT.ConcreteMajor
+
+val spot_concrete_b_forwarding_zero
+  : r:unit{ConcreteMajor.spot_major_room} ->
+    Lemma (ensures
+      (Cheney.cheney_promote
+        GC.SPOT.ConcreteMinor.spot_minor2
+        (ConcreteMajor.spot_major_heap r)
+        (ConcreteMajor.spot_major_fp r)
+        (GC.SPOT.ThreeObjects.spot_roots (ConcreteMajor.spot_c r))).fwd_map
+        GC.SPOT.Layout.b_minor == 0UL)
