spot/GC.SPOT.ConcreteFull.fsti
@@ -1,0 +1,139 @@
+module GC.SPOT.ConcreteFull
+
+module U64 = FStar.UInt64
+module Seq = FStar.Seq
+
+open FStar.Seq
+open GC.Spec.Base
+open GC.Gen.Base
+open GC.Gen.MinorHeap
+
+module Cheney = GC.Gen.Cheney
+module GenImpl = GC.Gen.Impl
+module ConcreteMajor = GC.SPOT.ConcreteMajor
+module ConcreteMinor = GC.SPOT.ConcreteMinor
+module ThreeObjects = GC.SPOT.ThreeObjects
+
+val spot_concrete_c_final_survives
+  : r:unit{ConcreteMajor.spot_major_room} ->
+    d2:minor_heap -> b2:U64.t ->
+    roots_out:seq U64.t -> ok:bool -> final_major:heap ->
+    st:seq obj_addr -> cap:nat ->
+    Lemma
+      (requires (
+        let result =
+          Cheney.cheney_collect_spec
+            ConcreteMinor.spot_minor2
+            (ConcreteMajor.spot_major_heap r)
+            (ConcreteMajor.spot_major_fp r)
+            (ThreeObjects.spot_roots (ConcreteMajor.spot_c r)) in
+        ok /\
+        GenImpl.gen_gc_roots_post
+          ConcreteMinor.spot_minor2
+          (ConcreteMajor.spot_major_heap r)
+          (ConcreteMajor.spot_major_fp r)
+          (ThreeObjects.spot_roots (ConcreteMajor.spot_c r))
+          roots_out st /\
+        GenImpl.gen_gc_heap_shape_post
+          d2 b2 result.mc_major final_major result.mc_fp st cap /\
+        GenImpl.gen_gc_reachable_subgraph_isomorphism_post
+          ConcreteMinor.spot_minor2
+          (ConcreteMajor.spot_major_heap r)
+          (ConcreteMajor.spot_major_fp r)
+          (ThreeObjects.spot_roots (ConcreteMajor.spot_c r))
+          ok final_major roots_out st))
+      (ensures Seq.mem (ConcreteMajor.spot_c r)
+        (GC.Spec.Fields.objects zero_addr final_major))
+
+val spot_concrete_a_prime_final_survives
+  : r:unit{ConcreteMajor.spot_major_room} ->
+    d2:minor_heap -> b2:U64.t ->
+    roots_out:seq U64.t -> ok:bool -> final_major:heap ->
+    st:seq obj_addr -> cap:nat ->
+    Lemma
+      (requires (
+        let result =
+          Cheney.cheney_collect_spec
+            ConcreteMinor.spot_minor2
+            (ConcreteMajor.spot_major_heap r)
+            (ConcreteMajor.spot_major_fp r)
+            (ThreeObjects.spot_roots (ConcreteMajor.spot_c r)) in
+        ok /\
+        GC.Gen.CheneyBFS.cheney_no_oom
+          ConcreteMinor.spot_minor2
+          (ConcreteMajor.spot_major_heap r)
+          (ConcreteMajor.spot_major_fp r)
+          (ThreeObjects.spot_roots (ConcreteMajor.spot_c r)) /\
+        GenImpl.gen_gc_roots_post
+          ConcreteMinor.spot_minor2
+          (ConcreteMajor.spot_major_heap r)
+          (ConcreteMajor.spot_major_fp r)
+          (ThreeObjects.spot_roots (ConcreteMajor.spot_c r))
+          roots_out st /\
+        GenImpl.gen_gc_heap_shape_post
+          d2 b2 result.mc_major final_major result.mc_fp st cap /\
+        GenImpl.gen_gc_reachable_subgraph_isomorphism_post
+          ConcreteMinor.spot_minor2
+          (ConcreteMajor.spot_major_heap r)
+          (ConcreteMajor.spot_major_fp r)
+          (ThreeObjects.spot_roots (ConcreteMajor.spot_c r))
+          ok final_major roots_out st))
+      (ensures (
+        let prom =
+          Cheney.cheney_promote
+            ConcreteMinor.spot_minor2
+            (ConcreteMajor.spot_major_heap r)
+            (ConcreteMajor.spot_major_fp r)
+            (ThreeObjects.spot_roots (ConcreteMajor.spot_c r)) in
+        exists (a_prime:obj_addr).
+          a_prime == prom.fwd_map GC.SPOT.Layout.a_minor /\
+          Seq.mem a_prime (GC.Spec.Fields.objects zero_addr final_major))
+      )
+
+val spot_concrete_c_field_final_points_to_a_prime
+  : r:unit{ConcreteMajor.spot_major_room} ->
+    d2:minor_heap -> b2:U64.t ->
+    roots_out:seq U64.t -> ok:bool -> final_major:heap ->
+    st:seq obj_addr -> cap:nat ->
+    Lemma
+      (requires (
+        let result =
+          Cheney.cheney_collect_spec
+            ConcreteMinor.spot_minor2
+            (ConcreteMajor.spot_major_heap r)
+            (ConcreteMajor.spot_major_fp r)
+            (ThreeObjects.spot_roots (ConcreteMajor.spot_c r)) in
+        ok /\
+        GC.Gen.CheneyBFS.cheney_no_oom
+          ConcreteMinor.spot_minor2
+          (ConcreteMajor.spot_major_heap r)
+          (ConcreteMajor.spot_major_fp r)
+          (ThreeObjects.spot_roots (ConcreteMajor.spot_c r)) /\
+        GenImpl.gen_gc_roots_post
+          ConcreteMinor.spot_minor2
+          (ConcreteMajor.spot_major_heap r)
+          (ConcreteMajor.spot_major_fp r)
+          (ThreeObjects.spot_roots (ConcreteMajor.spot_c r))
+          roots_out st /\
+        GenImpl.gen_gc_heap_shape_post
+          d2 b2 result.mc_major final_major result.mc_fp st cap /\
+        GenImpl.gen_gc_reachable_subgraph_isomorphism_post
+          ConcreteMinor.spot_minor2
+          (ConcreteMajor.spot_major_heap r)
+          (ConcreteMajor.spot_major_fp r)
+          (ThreeObjects.spot_roots (ConcreteMajor.spot_c r))
+          ok final_major roots_out st))
+      (ensures (
+        let prom =
+          Cheney.cheney_promote
+            ConcreteMinor.spot_minor2
+            (ConcreteMajor.spot_major_heap r)
+            (ConcreteMajor.spot_major_fp r)
+            (ThreeObjects.spot_roots (ConcreteMajor.spot_c r)) in
+        Seq.mem (ConcreteMajor.spot_c r)
+          (GC.Spec.Fields.objects zero_addr final_major) /\
+        exists (a_prime:obj_addr).
+          a_prime == prom.fwd_map GC.SPOT.Layout.a_minor /\
+          Seq.mem a_prime (GC.Spec.Fields.objects zero_addr final_major) /\
+          GC.Spec.Heap.read_word final_major (ConcreteMajor.spot_c_field1 r) ==
+            a_prime))
