spot/GC.SPOT.ConcreteScenarios.fst
@@ -1,0 +1,649 @@
+module GC.SPOT.ConcreteScenarios
+
+module U64 = FStar.UInt64
+module Seq = FStar.Seq
+
+open FStar.Seq
+open GC.Spec.Base
+open GC.Gen.Base
+open GC.Gen.MinorHeap
+
+module Layout = GC.SPOT.Layout
+module Preconditions = GC.SPOT.Preconditions
+module ThreeObjects = GC.SPOT.ThreeObjects
+module ConcreteMinor = GC.SPOT.ConcreteMinor
+module ConcreteMajor = GC.SPOT.ConcreteMajor
+module Postconditions = GC.SPOT.Postconditions
+module SpecHeap = GC.Spec.Heap
+module SpecObj = GC.Spec.Object
+module SpecFields = GC.Spec.Fields
+module GenInv = GC.Gen.HeapInvariant
+module Promote = GC.Gen.Promote
+module Cheney = GC.Gen.Cheney
+module CheneyBFS = GC.Gen.CheneyBFS
+module ConcreteForwarding = GC.SPOT.ConcreteForwarding
+module MinorFwd = GC.Gen.MinorCollectForwarding
+module MinorFwdHelpers = GC.Gen.MinorCollectForwarding.Helpers
+module RBridge = GC.Gen.ReachabilityBridge
+module UpdatePtrs = GC.Gen.Impl.UpdatePtrs
+module GenImpl = GC.Gen.Impl
+
+let spot_fwd_array : seq U64.t =
+  Seq.create UpdatePtrs.fwd_array_size 0UL
+
+#push-options "--z3rlimit 10 --fuel 0 --ifuel 0"
+let zero_not_minor_pointer ()
+  : Lemma (ensures ~(Promote.is_minor_pointer 0UL))
+  = assert_norm (Promote.is_minor_pointer 0UL == false)
+
+let zero_not_major_pointer ()
+  : Lemma (ensures ~(SpecFields.is_pointer_field 0UL))
+  =
+  zero_addr_above_2048 ();
+  assert (U64.v 0UL < U64.v zero_addr + U64.v mword)
+#pop-options
+
+#push-options "--z3rlimit 10 --fuel 0 --ifuel 0"
+let spot_fwd_array_zero ()
+  : Lemma (Preconditions.zero_forwarding_array spot_fwd_array)
+  =
+  FStar.Seq.Base.lemma_create_len UpdatePtrs.fwd_array_size 0UL;
+  assert (Seq.length spot_fwd_array == UpdatePtrs.fwd_array_size);
+  let aux (i: nat)
+    : Lemma (ensures i < Seq.length spot_fwd_array ==> Seq.index spot_fwd_array i == 0UL)
+    =
+    if i < Seq.length spot_fwd_array then begin
+      assert (i < UpdatePtrs.fwd_array_size);
+      FStar.Seq.Base.lemma_index_create UpdatePtrs.fwd_array_size 0UL i
+    end
+  in
+  FStar.Classical.forall_intro aux;
+  Preconditions.zero_forwarding_array_intro spot_fwd_array
+#pop-options
+
+#push-options "--z3rlimit 10 --fuel 0 --ifuel 0"
+let spot_c_slot_is_field1 (r: unit{ConcreteMajor.spot_major_room})
+  : Lemma (ThreeObjects.spot_c_to_a_slot (ConcreteMajor.spot_c r) ==
+           ConcreteMajor.spot_c_field1 r)
+  =
+  ConcreteMajor.spot_major_layout_facts r;
+  ThreeObjects.spot_c_to_a_slot_spec (ConcreteMajor.spot_c r);
+  assert (U64.v (ThreeObjects.spot_c_to_a_slot (ConcreteMajor.spot_c r)) ==
+          U64.v (ConcreteMajor.spot_c r) + 8);
+  assert (U64.v (ConcreteMajor.spot_c_field1 r) ==
+          U64.v (ConcreteMajor.spot_c r) + 8)
+#pop-options
+
+#push-options "--z3rlimit 10 --fuel 0 --ifuel 0"
+let spot_minor_major_fields_no_blue (r: unit{ConcreteMajor.spot_major_room})
+  : Lemma (GenInv.minor_major_fields_no_blue
+             ConcreteMinor.spot_minor2 (ConcreteMajor.spot_major_heap r))
+  =
+  let aux (obj: U64.t) (j: nat)
+    : Lemma
+        (requires
+          Seq.mem obj (minor_objects ConcreteMinor.spot_minor2) /\
+          j < minor_wosize ConcreteMinor.spot_minor2 obj)
+        (ensures
+          ~(SpecFields.is_pointer_field
+            (minor_read_field ConcreteMinor.spot_minor2 obj j)))
+    =
+    ConcreteMinor.spot_minor2_field_zero obj j;
+    zero_not_major_pointer ();
+    assert (minor_read_field ConcreteMinor.spot_minor2 obj j == 0UL)
+  in
+  FStar.Classical.forall_intro_2 (FStar.Classical.move_requires_2 aux);
+  GenInv.minor_major_fields_no_blue_no_pointer_fields
+    ConcreteMinor.spot_minor2 (ConcreteMajor.spot_major_heap r)
+#pop-options
+
+#push-options "--z3rlimit 10 --fuel 0 --ifuel 0"
+let spot_major_minor_fields_no_infix_targets (r: unit{ConcreteMajor.spot_major_room})
+  : Lemma (GenInv.major_minor_fields_no_infix_targets
+             ConcreteMinor.spot_minor2 (ConcreteMajor.spot_major_heap r))
+  =
+  let major = ConcreteMajor.spot_major_heap r in
+  let aux (obj: obj_addr) (j: nat)
+    : Lemma
+        (ensures
+          Seq.mem obj (SpecFields.objects zero_addr major) /\
+          ~(SpecObj.is_blue obj major) /\
+          ~(SpecObj.is_no_scan obj major) /\
+          j < U64.v (SpecObj.wosize_of_object obj major) /\
+          U64.v obj + j * 8 + 8 <= heap_size /\
+          (U64.v obj + j * 8) % 8 == 0 ==>
+          (let v = to_minor_offset
+             (SpecHeap.read_word major (U64.uint_to_t (U64.v obj + j * 8))) in
+           Promote.is_minor_pointer v ==> ~(is_infix_in_minor ConcreteMinor.spot_minor2 v)))
+    =
+    if Seq.mem obj (SpecFields.objects zero_addr major) /\
+       ~(SpecObj.is_blue obj major) /\
+       ~(SpecObj.is_no_scan obj major) /\
+       j < U64.v (SpecObj.wosize_of_object obj major) /\
+       U64.v obj + j * 8 + 8 <= heap_size /\
+       (U64.v obj + j * 8) % 8 == 0
+    then begin
+      ConcreteMajor.spot_major_object_cases r obj;
+      ConcreteMajor.spot_major_c_reads r;
+      ConcreteMajor.spot_major_free_reads r;
+      if obj = ConcreteMajor.spot_c r then begin
+        assert (U64.v (SpecObj.wosize_of_object obj major) == Layout.c_wosize);
+        assert (j < 2);
+        if j = 0 then begin
+          ConcreteMajor.spot_major_layout_facts r;
+          assert (U64.v obj == U64.v (ConcreteMajor.spot_c r));
+          assert (U64.v obj + j * 8 == U64.v (ConcreteMajor.spot_c r));
+          assert (U64.uint_to_t (U64.v obj + j * 8) == ConcreteMajor.spot_c_field0 r);
+          assert (SpecHeap.read_word major (U64.uint_to_t (U64.v obj + j * 8)) == 0UL);
+          zero_not_minor_pointer ()
+        end else begin
+          assert (j == Layout.c_to_a_field_index);
+          ConcreteMajor.spot_major_layout_facts r;
+          assert (U64.uint_to_t (U64.v obj + j * 8) == ConcreteMajor.spot_c_field1 r);
+          assert (SpecHeap.read_word major (U64.uint_to_t (U64.v obj + j * 8)) ==
+                  Layout.a_minor);
+          to_minor_offset_in_minor_range Layout.a_minor;
+          ConcreteMinor.spot_minor_a_not_infix ()
+        end
+      end else begin
+        assert (obj == ConcreteMajor.spot_free_obj r);
+        assert (SpecObj.is_blue obj major);
+        assert False
+      end
+    end
+  in
+  FStar.Classical.forall_intro_2 aux;
+  GenInv.major_minor_fields_no_infix_targets_intro
+    ConcreteMinor.spot_minor2 major
+#pop-options
+
+let spot_collection_heap_shape (r: unit{ConcreteMajor.spot_major_room})
+  : Lemma (GenInv.collection_heap_shape
+             ConcreteMinor.spot_minor2
+             (ConcreteMajor.spot_major_heap r)
+             (ConcreteMajor.spot_major_fp r))
+  =
+  ConcreteMajor.spot_major_heap_shape r;
+  ConcreteMinor.spot_minor_heap_shape ();
+  spot_minor_major_fields_no_blue r;
+  spot_major_minor_fields_no_infix_targets r;
+  GenInv.collection_heap_shape_intro
+    ConcreteMinor.spot_minor2
+    (ConcreteMajor.spot_major_heap r)
+    (ConcreteMajor.spot_major_fp r)
+
+#push-options "--z3rlimit 10 --fuel 0 --ifuel 0"
+let spot_ref_table_sound (r: unit{ConcreteMajor.spot_major_room})
+  : Lemma (UpdatePtrs.ref_table_sound
+             (ConcreteMajor.spot_major_heap r)
+             (ThreeObjects.spot_slots (ConcreteMajor.spot_c r)) 1)
+  =
+  let major = ConcreteMajor.spot_major_heap r in
+  spot_c_slot_is_field1 r;
+  ThreeObjects.spot_slots_len (ConcreteMajor.spot_c r);
+  assert (1 <= Seq.length (ThreeObjects.spot_slots (ConcreteMajor.spot_c r)));
+  ConcreteMajor.spot_major_objects r;
+  ConcreteMajor.spot_major_c_reads r;
+  ConcreteMajor.spot_major_layout_facts r;
+  let aux (i: nat)
+    : Lemma (ensures
+              i < 1 ==>
+              (let addr = U64.v (Seq.index (ThreeObjects.spot_slots (ConcreteMajor.spot_c r)) i) in
+               addr < heap_size /\ addr % 8 == 0 /\
+               (exists (obj: obj_addr) (j: nat).
+                 Seq.mem obj (SpecFields.objects zero_addr major) /\
+                 SpecObj.is_blue obj major = false /\
+                 SpecObj.is_no_scan obj major = false /\
+                 j < U64.v (SpecObj.wosize_of_object obj major) /\
+                 addr == U64.v obj + j * 8)))
+    =
+    if i < 1 then begin
+      assert (i == 0);
+      assert (i < Seq.length (ThreeObjects.spot_slots (ConcreteMajor.spot_c r)));
+      ThreeObjects.spot_slots_index (ConcreteMajor.spot_c r) i;
+      assert (Seq.index (ThreeObjects.spot_slots (ConcreteMajor.spot_c r)) i ==
+              ConcreteMajor.spot_c_field1 r);
+      assert (U64.v (ConcreteMajor.spot_c_field1 r) ==
+              U64.v (ConcreteMajor.spot_c r) + Layout.c_to_a_field_index * 8);
+      ThreeObjects.spot_roots_mem_c (ConcreteMajor.spot_c r);
+      ConcreteMajor.spot_major_c_mem r;
+      assert (Seq.mem (ConcreteMajor.spot_c r)
+        (SpecFields.objects zero_addr major));
+      assert (Layout.c_to_a_field_index < U64.v (SpecObj.wosize_of_object
+        (ConcreteMajor.spot_c r) major));
+      assert (exists (obj: obj_addr) (j: nat).
+        Seq.mem obj (SpecFields.objects zero_addr major) /\
+        SpecObj.is_blue obj major = false /\
+        SpecObj.is_no_scan obj major = false /\
+        j < U64.v (SpecObj.wosize_of_object obj major) /\
+        U64.v (ConcreteMajor.spot_c_field1 r) == U64.v obj + j * 8)
+    end
+  in
+  FStar.Classical.forall_intro aux
+#pop-options
+
+#push-options "--z3rlimit 10 --fuel 0 --ifuel 0"
+let spot_ref_table_covers_minor_ptrs (r: unit{ConcreteMajor.spot_major_room})
+  : Lemma (UpdatePtrs.ref_table_covers_minor_ptrs
+             (ConcreteMajor.spot_major_heap r)
+             (ThreeObjects.spot_slots (ConcreteMajor.spot_c r)) 1)
+  =
+  let major = ConcreteMajor.spot_major_heap r in
+  spot_c_slot_is_field1 r;
+  ThreeObjects.spot_slots_len (ConcreteMajor.spot_c r);
+  assert (1 <= Seq.length (ThreeObjects.spot_slots (ConcreteMajor.spot_c r)));
+  ConcreteMajor.spot_major_objects r;
+  ConcreteMajor.spot_major_c_reads r;
+  ConcreteMajor.spot_major_free_reads r;
+  let aux (obj: obj_addr) (j: nat)
+    : Lemma
+        (ensures
+          Seq.mem obj (SpecFields.objects zero_addr major) /\
+          SpecObj.is_blue obj major = false /\
+          SpecObj.is_no_scan obj major = false /\
+          j < U64.v (SpecObj.wosize_of_object obj major) /\
+          U64.v obj + j * 8 + 8 <= heap_size /\
+          (let field_val =
+            to_minor_offset
+              (SpecHeap.read_word major (U64.uint_to_t (U64.v obj + j * 8))) in
+           Promote.is_minor_pointer field_val) ==>
+          (exists (i: nat).
+            i < 1 /\
+            U64.v (Seq.index (ThreeObjects.spot_slots (ConcreteMajor.spot_c r)) i) ==
+              U64.v obj + j * 8))
+    =
+    if Seq.mem obj (SpecFields.objects zero_addr major) /\
+       SpecObj.is_blue obj major = false /\
+       SpecObj.is_no_scan obj major = false /\
+       j < U64.v (SpecObj.wosize_of_object obj major) /\
+       U64.v obj + j * 8 + 8 <= heap_size /\
+       (let field_val =
+          to_minor_offset
+            (SpecHeap.read_word major (U64.uint_to_t (U64.v obj + j * 8))) in
+        Promote.is_minor_pointer field_val)
+    then begin
+      ConcreteMajor.spot_major_object_cases r obj;
+      if obj = ConcreteMajor.spot_c r then begin
+        ConcreteMajor.spot_major_layout_facts r;
+        assert (obj == ConcreteMajor.spot_c r);
+        assert (U64.v (SpecObj.wosize_of_object obj major) == Layout.c_wosize);
+        assert (j < 2);
+        if j = 0 then begin
+          assert (j == 0);
+          assert (U64.v (ConcreteMajor.spot_c_field0 r) == U64.v obj + j * 8);
+          assert (U64.uint_to_t (U64.v obj + j * 8) == ConcreteMajor.spot_c_field0 r);
+          assert (SpecHeap.read_word major (U64.uint_to_t (U64.v obj + j * 8)) == 0UL);
+          zero_not_minor_pointer ();
+          assert False
+        end else begin
+          assert (j <> 0);
+          assert (j == Layout.c_to_a_field_index);
+          assert (U64.v (ConcreteMajor.spot_c_field1 r) == U64.v obj + j * 8);
+          assert (U64.uint_to_t (U64.v obj + j * 8) == ConcreteMajor.spot_c_field1 r);
+          ThreeObjects.spot_slots_index (ConcreteMajor.spot_c r) 0;
+          assert (Seq.index (ThreeObjects.spot_slots (ConcreteMajor.spot_c r)) 0 ==
+                  ConcreteMajor.spot_c_field1 r);
+          assert (U64.v (Seq.index (ThreeObjects.spot_slots (ConcreteMajor.spot_c r)) 0) ==
+                  U64.v obj + j * 8);
+          assert (exists (i: nat).
+            i < 1 /\
+            U64.v (Seq.index (ThreeObjects.spot_slots (ConcreteMajor.spot_c r)) i) ==
+              U64.v obj + j * 8)
+        end
+      end else begin
+        assert (obj == ConcreteMajor.spot_free_obj r);
+        ConcreteMajor.spot_major_free_reads r;
+        assert (SpecObj.is_blue obj major);
+        assert False
+      end
+    end
+  in
+  FStar.Classical.forall_intro_2 aux
+#pop-options
+
+#push-options "--z3rlimit 10 --fuel 0 --ifuel 0"
+let spot_remembered_targets_in_roots (r: unit{ConcreteMajor.spot_major_room})
+  : Lemma (MinorFwd.remembered_targets_in_roots
+             (ConcreteMajor.spot_major_heap r)
+             (ThreeObjects.spot_roots (ConcreteMajor.spot_c r))
+             (ThreeObjects.spot_slots (ConcreteMajor.spot_c r)) 1)
+  =
+  let major = ConcreteMajor.spot_major_heap r in
+  spot_c_slot_is_field1 r;
+  ThreeObjects.spot_slots_len (ConcreteMajor.spot_c r);
+  assert (1 <= Seq.length (ThreeObjects.spot_slots (ConcreteMajor.spot_c r)));
+  ConcreteMajor.spot_major_c_reads r;
+  let aux (i: nat)
+    : Lemma (ensures
+              i < 1 ==>
+              U64.v (Seq.index (ThreeObjects.spot_slots (ConcreteMajor.spot_c r)) i) < heap_size /\
+              U64.v (Seq.index (ThreeObjects.spot_slots (ConcreteMajor.spot_c r)) i) % U64.v mword == 0 /\
+              (let slot = (Seq.index (ThreeObjects.spot_slots (ConcreteMajor.spot_c r)) i <: hp_addr) in
+               let v = to_minor_offset (SpecHeap.read_word major slot) in
+               Promote.is_minor_pointer v ==> Seq.mem v (ThreeObjects.spot_roots (ConcreteMajor.spot_c r))))
+    =
+    if i < 1 then begin
+      assert (i == 0);
+      assert (i < Seq.length (ThreeObjects.spot_slots (ConcreteMajor.spot_c r)));
+      ThreeObjects.spot_slots_index (ConcreteMajor.spot_c r) i;
+      assert (Seq.index (ThreeObjects.spot_slots (ConcreteMajor.spot_c r)) i ==
+              ConcreteMajor.spot_c_field1 r);
+      assert (SpecHeap.read_word major (ConcreteMajor.spot_c_field1 r) == Layout.a_minor);
+      to_minor_offset_in_minor_range Layout.a_minor;
+      ThreeObjects.spot_roots_mem_a (ConcreteMajor.spot_c r)
+    end
+  in
+  FStar.Classical.forall_intro aux;
+  MinorFwdHelpers.remembered_targets_in_roots_intro_by_slots
+    major (ThreeObjects.spot_roots (ConcreteMajor.spot_c r))
+    (ThreeObjects.spot_slots (ConcreteMajor.spot_c r)) 1
+#pop-options
+
+#push-options "--z3rlimit 10 --fuel 0 --ifuel 0"
+let spot_major_field_zero_no_minor (r: unit{ConcreteMajor.spot_major_room})
+  : Lemma (RBridge.major_field_zero_no_minor
+             ConcreteMinor.spot_minor2 (ConcreteMajor.spot_major_heap r))
+  =
+  let major = ConcreteMajor.spot_major_heap r in
+  let aux (src: obj_addr)
+    : Lemma
+        (requires
+          Seq.mem src (SpecFields.objects zero_addr major) /\
+          ~(SpecObj.is_no_scan src major) /\
+          U64.v src + 8 <= heap_size)
+        (ensures
+          (let v = to_minor_offset (SpecHeap.read_word major (U64.uint_to_t (U64.v src))) in
+           ~(Promote.is_minor_pointer v)))
+    =
+    ConcreteMajor.spot_major_object_cases r src;
+    ConcreteMajor.spot_major_c_reads r;
+    ConcreteMajor.spot_major_free_reads r;
+    if src = ConcreteMajor.spot_c r then begin
+      ConcreteMajor.spot_major_layout_facts r;
+      assert (src == ConcreteMajor.spot_c r);
+      assert (U64.v (ConcreteMajor.spot_c_field0 r) == U64.v src);
+      assert (U64.uint_to_t (U64.v src) == ConcreteMajor.spot_c_field0 r);
+      assert (SpecHeap.read_word major (U64.uint_to_t (U64.v src)) == 0UL);
+      zero_not_minor_pointer ()
+    end else begin
+      assert (src == ConcreteMajor.spot_free_obj r);
+      ConcreteMajor.spot_major_layout_facts r;
+      assert (0 < ConcreteMajor.spot_free_wosize r);
+      assert (U64.v (ConcreteMajor.spot_free_obj r) + 0 * 8 + 8 <= heap_size);
+      ConcreteMajor.spot_major_free_field_read r 0;
+      assert (SpecHeap.read_word major (U64.uint_to_t (U64.v src)) == 0UL);
+      zero_not_minor_pointer ()
+    end
+  in
+  FStar.Classical.forall_intro (FStar.Classical.move_requires aux)
+#pop-options
+
+#push-options "--z3rlimit 10 --fuel 0 --ifuel 0"
+let spot_roots_valid_nonblue (r: unit{ConcreteMajor.spot_major_room})
+  : Lemma (RBridge.roots_valid_nonblue
+             (ThreeObjects.spot_roots (ConcreteMajor.spot_c r))
+             (ConcreteMajor.spot_major_heap r))
+  =
+  let major = ConcreteMajor.spot_major_heap r in
+  let aux (root: U64.t)
+    : Lemma
+        (ensures
+          Seq.mem root (ThreeObjects.spot_roots (ConcreteMajor.spot_c r)) /\
+          ~(Promote.is_minor_pointer root) /\
+          is_val_addr root /\
+          Seq.mem (root <: obj_addr) (SpecFields.objects zero_addr major) ==>
+          ~(SpecObj.is_blue (root <: obj_addr) major))
+    =
+    if Seq.mem root (ThreeObjects.spot_roots (ConcreteMajor.spot_c r)) /\
+       ~(Promote.is_minor_pointer root) /\
+       is_val_addr root /\
+       Seq.mem (root <: obj_addr) (SpecFields.objects zero_addr major)
+    then begin
+      ThreeObjects.spot_roots_cases (ConcreteMajor.spot_c r) root;
+      if root = (ConcreteMajor.spot_c r <: U64.t) then begin
+        assert ((root <: obj_addr) == ConcreteMajor.spot_c r);
+        ConcreteMajor.spot_major_c_reads r
+      end else begin
+        assert (root == Layout.a_minor);
+        if root = Layout.a_minor then begin
+          Layout.a_minor_is_minor_pointer ();
+          assert False
+        end else begin
+          assert False
+        end
+      end
+    end
+  in
+  FStar.Classical.forall_intro aux
+#pop-options
+
+#push-options "--z3rlimit 10 --fuel 0 --ifuel 0"
+let spot_roots_valid_for_minor_collection (r: unit{ConcreteMajor.spot_major_room})
+  : Lemma (MinorFwd.roots_valid_for_minor_collection
+             ConcreteMinor.spot_minor2
+             (ConcreteMajor.spot_major_heap r)
+             (ThreeObjects.spot_roots (ConcreteMajor.spot_c r)))
+  =
+  let major = ConcreteMajor.spot_major_heap r in
+  let aux (root: U64.t)
+    : Lemma
+        (requires Seq.mem root (ThreeObjects.spot_roots (ConcreteMajor.spot_c r)))
+        (ensures
+          ((Promote.is_minor_pointer root ==>
+            Seq.mem root (minor_objects ConcreteMinor.spot_minor2) /\
+            minor_wosize ConcreteMinor.spot_minor2 root > 0) /\
+           (~(Promote.is_minor_pointer root) ==>
+            is_val_addr root /\
+            Seq.mem (root <: obj_addr) (SpecFields.objects zero_addr major) /\
+            ~(SpecObj.is_blue (root <: obj_addr) major))))
+    =
+    ThreeObjects.spot_roots_cases (ConcreteMajor.spot_c r) root;
+    if root = (ConcreteMajor.spot_c r <: U64.t) then begin
+      ConcreteMajor.spot_major_c_reads r;
+      ConcreteMajor.spot_major_c_mem r;
+      assert ((root <: obj_addr) == ConcreteMajor.spot_c r);
+      assert (Seq.mem (ConcreteMajor.spot_c r) (SpecFields.objects zero_addr major));
+      RBridge.major_object_not_minor_pointer major (ConcreteMajor.spot_c r)
+    end else begin
+      assert (root == Layout.a_minor);
+      if root = Layout.a_minor then begin
+        Layout.a_minor_is_minor_pointer ();
+        ConcreteMinor.spot_minor_two_object_layout ()
+      end else begin
+        assert False
+      end
+    end
+  in
+  FStar.Classical.forall_intro (FStar.Classical.move_requires aux)
+#pop-options
+
+let spot_concrete_minor_collect_full_pre (r: unit{ConcreteMajor.spot_major_room})
+  : Lemma
+      (Preconditions.minor_collect_full_pre
+        ConcreteMinor.spot_minor2
+        (ConcreteMajor.spot_major_heap r)
+        (ConcreteMajor.spot_major_fp r)
+        (ThreeObjects.spot_roots (ConcreteMajor.spot_c r))
+        spot_fwd_array
+        (ThreeObjects.spot_slots (ConcreteMajor.spot_c r))
+        1)
+  =
+  spot_collection_heap_shape r;
+  spot_fwd_array_zero ();
+  spot_ref_table_sound r;
+  spot_ref_table_covers_minor_ptrs r;
+  ThreeObjects.spot_slots_singleton_distinct (ConcreteMajor.spot_c r);
+  spot_remembered_targets_in_roots r;
+  spot_major_field_zero_no_minor r;
+  spot_roots_valid_nonblue r;
+  spot_roots_valid_for_minor_collection r;
+  Preconditions.minor_collect_full_pre_intro
+    ConcreteMinor.spot_minor2
+    (ConcreteMajor.spot_major_heap r)
+    (ConcreteMajor.spot_major_fp r)
+    (ThreeObjects.spot_roots (ConcreteMajor.spot_c r))
+    spot_fwd_array
+    (ThreeObjects.spot_slots (ConcreteMajor.spot_c r))
+    1
+
+let spot_concrete_minor_scenario_pre_from_no_oom
+  (r: unit{ConcreteMajor.spot_major_room})
+  : Lemma
+      (requires
+        CheneyBFS.cheney_no_oom
+          ConcreteMinor.spot_minor2
+          (ConcreteMajor.spot_major_heap r)
+          (ConcreteMajor.spot_major_fp r)
+          (ThreeObjects.spot_roots (ConcreteMajor.spot_c r)))
+      (ensures
+        ThreeObjects.spot_minor_scenario_pre
+          ConcreteMinor.spot_minor2
+          (ConcreteMajor.spot_major_heap r)
+          (ConcreteMajor.spot_major_fp r)
+          (ConcreteMajor.spot_c r)
+          spot_fwd_array)
+  =
+  spot_concrete_minor_collect_full_pre r;
+  ConcreteMajor.spot_major_objects r;
+  ConcreteMajor.spot_major_c_mem r;
+  ConcreteMajor.spot_major_c_reads r;
+  ConcreteMinor.spot_minor_two_object_layout ();
+  spot_c_slot_is_field1 r;
+  RBridge.major_object_not_minor_pointer
+    (ConcreteMajor.spot_major_heap r) (ConcreteMajor.spot_c r);
+  assert (U64.v (SpecObj.wosize_of_object (ConcreteMajor.spot_c r)
+                   (ConcreteMajor.spot_major_heap r)) == Layout.c_wosize);
+  assert (U64.v (SpecObj.wosize_of_object (ConcreteMajor.spot_c r)
+                   (ConcreteMajor.spot_major_heap r)) >
+          Layout.c_to_a_field_index);
+  assert (SpecHeap.read_word (ConcreteMajor.spot_major_heap r)
+    (ThreeObjects.spot_c_to_a_slot (ConcreteMajor.spot_c r)) ==
+    Layout.a_minor);
+  assert (minor_wosize ConcreteMinor.spot_minor2 Layout.a_minor > 0);
+  assert (minor_wosize ConcreteMinor.spot_minor2 Layout.b_minor > 0);
+  ThreeObjects.spot_minor_scenario_pre_intro_from_c_to_a
+    ConcreteMinor.spot_minor2
+    (ConcreteMajor.spot_major_heap r)
+    (ConcreteMajor.spot_major_fp r)
+    (ConcreteMajor.spot_c r)
+    spot_fwd_array
+
+let spot_concrete_gen_gc_pre_from_stack
+  (r: unit{ConcreteMajor.spot_major_room}) (st: seq obj_addr) (cap: nat)
+  : Lemma
+      (requires
+        (let result =
+          Cheney.cheney_collect_spec
+            ConcreteMinor.spot_minor2
+            (ConcreteMajor.spot_major_heap r)
+            (ConcreteMajor.spot_major_fp r)
+            (ThreeObjects.spot_roots (ConcreteMajor.spot_c r)) in
+        GenInv.major_stack_shape result.mc_major st cap /\
+        GenImpl.roots_match_stack result.mc_roots st))
+      (ensures
+        Preconditions.gen_gc_pre
+          ConcreteMinor.spot_minor2
+          (ConcreteMajor.spot_major_heap r)
+          (ConcreteMajor.spot_major_fp r)
+          (ThreeObjects.spot_roots (ConcreteMajor.spot_c r))
+          spot_fwd_array
+          (ThreeObjects.spot_slots (ConcreteMajor.spot_c r))
+          1 st cap)
+  =
+  spot_concrete_minor_collect_full_pre r;
+  Preconditions.gen_gc_pre_intro
+    ConcreteMinor.spot_minor2
+    (ConcreteMajor.spot_major_heap r)
+    (ConcreteMajor.spot_major_fp r)
+    (ThreeObjects.spot_roots (ConcreteMajor.spot_c r))
+    spot_fwd_array
+    (ThreeObjects.spot_slots (ConcreteMajor.spot_c r))
+    1 st cap
+
+let spot_concrete_a_promoted_from_no_oom (r: unit{ConcreteMajor.spot_major_room})
+  : Lemma
+      (requires
+        CheneyBFS.cheney_no_oom
+          ConcreteMinor.spot_minor2
+          (ConcreteMajor.spot_major_heap r)
+          (ConcreteMajor.spot_major_fp r)
+          (ThreeObjects.spot_roots (ConcreteMajor.spot_c r)))
+      (ensures (
+        let prom =
+          Cheney.cheney_promote
+            ConcreteMinor.spot_minor2
+            (ConcreteMajor.spot_major_heap r)
+            (ConcreteMajor.spot_major_fp r)
+            (ThreeObjects.spot_roots (ConcreteMajor.spot_c r)) in
+        Postconditions.promoted_image
+          ConcreteMinor.spot_minor2
+          (ConcreteMajor.spot_major_heap r)
+          (ConcreteMajor.spot_major_fp r)
+          (ThreeObjects.spot_roots (ConcreteMajor.spot_c r))
+          Layout.a_minor
+          (prom.fwd_map Layout.a_minor)))
+  =
+  spot_concrete_minor_scenario_pre_from_no_oom r;
+  ThreeObjects.spot_a_promoted
+    ConcreteMinor.spot_minor2
+    (ConcreteMajor.spot_major_heap r)
+    (ConcreteMajor.spot_major_fp r)
+    (ConcreteMajor.spot_c r)
+    spot_fwd_array
+
+let spot_concrete_c_field_rewritten_from_no_oom
+  (r: unit{ConcreteMajor.spot_major_room})
+  : Lemma
+      (requires
+        CheneyBFS.cheney_no_oom
+          ConcreteMinor.spot_minor2
+          (ConcreteMajor.spot_major_heap r)
+          (ConcreteMajor.spot_major_fp r)
+          (ThreeObjects.spot_roots (ConcreteMajor.spot_c r)))
+      (ensures (
+        let prom =
+          Cheney.cheney_promote
+            ConcreteMinor.spot_minor2
+            (ConcreteMajor.spot_major_heap r)
+            (ConcreteMajor.spot_major_fp r)
+            (ThreeObjects.spot_roots (ConcreteMajor.spot_c r)) in
+        let res =
+          Cheney.cheney_collect_spec
+            ConcreteMinor.spot_minor2
+            (ConcreteMajor.spot_major_heap r)
+            (ConcreteMajor.spot_major_fp r)
+            (ThreeObjects.spot_roots (ConcreteMajor.spot_c r)) in
+        Postconditions.promoted_image
+          ConcreteMinor.spot_minor2
+          (ConcreteMajor.spot_major_heap r)
+          (ConcreteMajor.spot_major_fp r)
+          (ThreeObjects.spot_roots (ConcreteMajor.spot_c r))
+          Layout.a_minor
+          (prom.fwd_map Layout.a_minor) /\
+        SpecHeap.read_word res.mc_major (ConcreteMajor.spot_c_field1 r) ==
+          prom.fwd_map Layout.a_minor))
+  =
+  spot_concrete_minor_scenario_pre_from_no_oom r;
+  ThreeObjects.spot_c_field_rewritten_to_a_prime
+    ConcreteMinor.spot_minor2
+    (ConcreteMajor.spot_major_heap r)
+    (ConcreteMajor.spot_major_fp r)
+    (ConcreteMajor.spot_c r)
+    spot_fwd_array;
+  spot_c_slot_is_field1 r
+
+let spot_concrete_b_not_promoted (r: unit{ConcreteMajor.spot_major_room})
+  : Lemma (ensures
+      Postconditions.minor_not_promoted
+        ConcreteMinor.spot_minor2
+        (ConcreteMajor.spot_major_heap r)
+        (ConcreteMajor.spot_major_fp r)
+        (ThreeObjects.spot_roots (ConcreteMajor.spot_c r))
+        Layout.b_minor)
+  =
+  ConcreteForwarding.spot_concrete_b_forwarding_zero r;
+  ThreeObjects.spot_b_not_promoted_from_forwarding_zero
+    ConcreteMinor.spot_minor2
+    (ConcreteMajor.spot_major_heap r)
+    (ConcreteMajor.spot_major_fp r)
+    (ConcreteMajor.spot_c r)
