spot/GC.SPOT.ConcreteScenarios.fsti
@@ -1,0 +1,146 @@
+module GC.SPOT.ConcreteScenarios
+
+module U64 = FStar.UInt64
+module Seq = FStar.Seq
+
+open FStar.Seq
+open GC.Spec.Base
+open GC.Gen.Base
+
+module Cheney = GC.Gen.Cheney
+module GenImpl = GC.Gen.Impl
+module GenInv = GC.Gen.HeapInvariant
+module Preconditions = GC.SPOT.Preconditions
+module ThreeObjects = GC.SPOT.ThreeObjects
+module ConcreteMajor = GC.SPOT.ConcreteMajor
+module ConcreteMinor = GC.SPOT.ConcreteMinor
+module UpdatePtrs = GC.Gen.Impl.UpdatePtrs
+
+val spot_fwd_array : seq U64.t
+
+val spot_fwd_array_zero : unit ->
+  Lemma (ensures Preconditions.zero_forwarding_array spot_fwd_array)
+
+val spot_c_slot_is_field1
+  : r:unit{ConcreteMajor.spot_major_room} ->
+    Lemma (ensures
+      ThreeObjects.spot_c_to_a_slot (ConcreteMajor.spot_c r) ==
+      ConcreteMajor.spot_c_field1 r)
+
+val spot_concrete_minor_collect_full_pre
+  : r:unit{ConcreteMajor.spot_major_room} ->
+    Lemma (ensures
+      Preconditions.minor_collect_full_pre
+        ConcreteMinor.spot_minor2
+        (ConcreteMajor.spot_major_heap r)
+        (ConcreteMajor.spot_major_fp r)
+        (ThreeObjects.spot_roots (ConcreteMajor.spot_c r))
+        spot_fwd_array
+        (ThreeObjects.spot_slots (ConcreteMajor.spot_c r))
+        1)
+
+val spot_concrete_minor_scenario_pre_from_no_oom
+  : r:unit{ConcreteMajor.spot_major_room} ->
+    Lemma
+      (requires
+        GC.Gen.CheneyBFS.cheney_no_oom
+          ConcreteMinor.spot_minor2
+          (ConcreteMajor.spot_major_heap r)
+          (ConcreteMajor.spot_major_fp r)
+          (ThreeObjects.spot_roots (ConcreteMajor.spot_c r)))
+      (ensures
+        ThreeObjects.spot_minor_scenario_pre
+          ConcreteMinor.spot_minor2
+          (ConcreteMajor.spot_major_heap r)
+          (ConcreteMajor.spot_major_fp r)
+          (ConcreteMajor.spot_c r)
+          spot_fwd_array)
+
+val spot_concrete_gen_gc_pre_from_stack
+  : r:unit{ConcreteMajor.spot_major_room} ->
+    st:seq obj_addr -> cap:nat ->
+    Lemma
+      (requires
+        (let result =
+          Cheney.cheney_collect_spec
+            ConcreteMinor.spot_minor2
+            (ConcreteMajor.spot_major_heap r)
+            (ConcreteMajor.spot_major_fp r)
+            (ThreeObjects.spot_roots (ConcreteMajor.spot_c r)) in
+        GenInv.major_stack_shape result.mc_major st cap /\
+        GenImpl.roots_match_stack result.mc_roots st))
+      (ensures
+        Preconditions.gen_gc_pre
+          ConcreteMinor.spot_minor2
+          (ConcreteMajor.spot_major_heap r)
+          (ConcreteMajor.spot_major_fp r)
+          (ThreeObjects.spot_roots (ConcreteMajor.spot_c r))
+          spot_fwd_array
+          (ThreeObjects.spot_slots (ConcreteMajor.spot_c r))
+          1 st cap)
+
+val spot_concrete_a_promoted_from_no_oom
+  : r:unit{ConcreteMajor.spot_major_room} ->
+    Lemma
+      (requires
+        GC.Gen.CheneyBFS.cheney_no_oom
+          ConcreteMinor.spot_minor2
+          (ConcreteMajor.spot_major_heap r)
+          (ConcreteMajor.spot_major_fp r)
+          (ThreeObjects.spot_roots (ConcreteMajor.spot_c r)))
+      (ensures (
+        let prom =
+          Cheney.cheney_promote
+            ConcreteMinor.spot_minor2
+            (ConcreteMajor.spot_major_heap r)
+            (ConcreteMajor.spot_major_fp r)
+            (ThreeObjects.spot_roots (ConcreteMajor.spot_c r)) in
+        GC.SPOT.Postconditions.promoted_image
+          ConcreteMinor.spot_minor2
+          (ConcreteMajor.spot_major_heap r)
+          (ConcreteMajor.spot_major_fp r)
+          (ThreeObjects.spot_roots (ConcreteMajor.spot_c r))
+          GC.SPOT.Layout.a_minor
+          (prom.fwd_map GC.SPOT.Layout.a_minor)))
+
+val spot_concrete_c_field_rewritten_from_no_oom
+  : r:unit{ConcreteMajor.spot_major_room} ->
+    Lemma
+      (requires
+        GC.Gen.CheneyBFS.cheney_no_oom
+          ConcreteMinor.spot_minor2
+          (ConcreteMajor.spot_major_heap r)
+          (ConcreteMajor.spot_major_fp r)
+          (ThreeObjects.spot_roots (ConcreteMajor.spot_c r)))
+      (ensures (
+        let prom =
+          Cheney.cheney_promote
+            ConcreteMinor.spot_minor2
+            (ConcreteMajor.spot_major_heap r)
+            (ConcreteMajor.spot_major_fp r)
+            (ThreeObjects.spot_roots (ConcreteMajor.spot_c r)) in
+        let res =
+          Cheney.cheney_collect_spec
+            ConcreteMinor.spot_minor2
+            (ConcreteMajor.spot_major_heap r)
+            (ConcreteMajor.spot_major_fp r)
+            (ThreeObjects.spot_roots (ConcreteMajor.spot_c r)) in
+        GC.SPOT.Postconditions.promoted_image
+          ConcreteMinor.spot_minor2
+          (ConcreteMajor.spot_major_heap r)
+          (ConcreteMajor.spot_major_fp r)
+          (ThreeObjects.spot_roots (ConcreteMajor.spot_c r))
+          GC.SPOT.Layout.a_minor
+          (prom.fwd_map GC.SPOT.Layout.a_minor) /\
+        GC.Spec.Heap.read_word res.mc_major (ConcreteMajor.spot_c_field1 r) ==
+          prom.fwd_map GC.SPOT.Layout.a_minor))
+
+val spot_concrete_b_not_promoted
+  : r:unit{ConcreteMajor.spot_major_room} ->
+    Lemma (ensures
+      GC.SPOT.Postconditions.minor_not_promoted
+        ConcreteMinor.spot_minor2
+        (ConcreteMajor.spot_major_heap r)
+        (ConcreteMajor.spot_major_fp r)
+        (ThreeObjects.spot_roots (ConcreteMajor.spot_c r))
+        GC.SPOT.Layout.b_minor)
